treat symtbl as an oracle in module safety

common/SmallstepLinkingSafe.v
@@ -26,7 +26,7 @@ Definition safe {liA liB st} (L: lts liA liB st) (s: st) : Prop :=
 the original safe/partial_safe is identical to the composed
 safe/partial_safe *)
 
-Record lts_safe {liA liB S} se (L: lts liA liB S) (IA: invariant liA) (IB: invariant liB) (SI: _ -> S -> Prop) w :=
+Record lts_safe {liA liB S} se (L: lts liA liB S) (IA: invariant liA) (IB: invariant liB) (SI: _ -> S -> Prop) wI :=
   {
     step_safe s t s' (REACH: reachable L s):
       (* SI L s -> *)
@@ -34,7 +34,7 @@ Record lts_safe {liA liB S} se (L: lts liA liB S) (IA: invariant liA) (IB: invar
       SI L s';
     initial_safe q:
       valid_query L q = true ->
-      query_inv IB w q ->
+      query_inv IB wI q ->
       (* initial_progress *)
       (exists s, initial_state L q s)
       (* initial_safe *)
@@ -49,12 +49,13 @@ Record lts_safe {liA liB S} se (L: lts liA liB S) (IA: invariant liA) (IB: invar
                    /\ (forall s', after_external L s r s' -> SI L s');
     final_safe s r (REACH: reachable L s):
       final_state L s r ->
-      reply_inv IB w r;
+      reply_inv IB wI r;
   }.
 
 
-Definition module_safe {liA liB} (L: semantics liA liB) (IA IB: invariant _) SI :=
-  forall w se,
+(* se as an oracle, is it correct? *)
+Definition module_safe {liA liB} (L: semantics liA liB) (IA IB: invariant _) SI se :=
+  forall w,
     Genv.valid_for (skel L) se ->
     symtbl_inv IB w se ->
     lts_safe se (L se) IA IB SI w.
@@ -66,7 +67,7 @@ Lemma safe_internal {li} (I: invariant li) L1 L2: forall i sk se s k w,
       (VALID: Genv.valid_for (skel (SmallstepLinking.semantics L sk)) se)
       (INV : symtbl_inv I w se)
       (VALIDSE: forall i, Genv.valid_for (skel (L i)) se)
-      (SAFE: forall i, module_safe (L i) I I safe)
+      (SAFE: forall i, module_safe (L i) I I safe se)
       (STSAFE: safe (L i se) s)
       (WFSTATE: wf_state L se (st L i s :: k)),
       safe (SmallstepLinking.semantics L sk se) (st L i s :: k).
@@ -80,27 +81,27 @@ Proof.
        right. right.
        (* s0 in in at_external state *)
        inv WFSTATE. subst_dep. inv H3. inv H2. subst_dep.
-       generalize (external_safe _ _ _ _ _ _ (SAFE i0 _ _ (VALIDSE i0) INV) s0 q H5 H3).
+       generalize (external_safe _ _ _ _ _ _ (SAFE i0 _ (VALIDSE i0) INV) s0 q H5 H3).
        intros (wA & SYMBINV & QINV & AFTER).
-       generalize (final_safe _ _ _ _ _ _ (SAFE i _ _ (VALIDSE i) SYMBINV) _ _ H1 FINAL).
+       generalize (final_safe _ _ _ _ _ _ (SAFE i _ (VALIDSE i) SYMBINV) _ _ H1 FINAL).
        intros WR.
        generalize (AFTER _ WR).
        intros ((s0' & AFTER1) & SAFTER).
        do 2 eexists.
        eapply step_pop; eauto.
   * inv WFSTATE. subst_dep.
-    generalize (external_safe _ _ _ _ _ _ (SAFE i _ _ (VALIDSE i) INV) s q H1 EXT).
+    generalize (external_safe _ _ _ _ _ _ (SAFE i _ (VALIDSE i) INV) s q H1 EXT).
     intros (wA & SYMBINV & QINV & AFTER).
     destruct (valid_query (L i se) q) eqn: VQ1.
     -- right. right.
-       generalize (initial_safe _ _ _ _ _ _ (SAFE i _ _ (VALIDSE i) SYMBINV) _ VQ1 QINV).
+       generalize (initial_safe _ _ _ _ _ _ (SAFE i _ (VALIDSE i) SYMBINV) _ VQ1 QINV).
        intros ((initS & INIT) & INITSAFE).
        do 2 eexists.
        eapply step_push; eauto.
     -- destruct i; simpl in *.
        ++ destruct (valid_query (L2 se) q) eqn: VQ2.
           ** right. right.
-             generalize (initial_safe _ _ _ _ _ _ (SAFE false _ _ (VALIDSE false) SYMBINV) _ VQ2 QINV).
+             generalize (initial_safe _ _ _ _ _ _ (SAFE false _ (VALIDSE false) SYMBINV) _ VQ2 QINV).
              intros ((initS & INIT) & INITSAFE).
              do 2 eexists.
              eapply step_push. eauto.
@@ -112,7 +113,7 @@ Proof.
              intros. destruct j; simpl; auto.
        ++  destruct (valid_query (L1 se) q) eqn: VQ2.
            ** right. right.
-              generalize (initial_safe _ _ _ _ _ _ (SAFE true _ _ (VALIDSE true) SYMBINV) _ VQ2 QINV).
+              generalize (initial_safe _ _ _ _ _ _ (SAFE true _ (VALIDSE true) SYMBINV) _ VQ2 QINV).
               intros ((initS & INIT) & INITSAFE).
               do 2 eexists.
               eapply step_push. eauto.
@@ -126,23 +127,23 @@ Proof.
     eapply step_internal. simpl. eauto.
 Qed.
   
-Lemma compose_safety {li} (I: invariant li) L1 L2 L:
-  module_safe L1 I I safe ->
-  module_safe L2 I I safe ->
+Lemma compose_safety {li} (I: invariant li) L1 L2 L se:
+  module_safe L1 I I safe se ->
+  module_safe L2 I I safe se ->
   compose L1 L2 = Some L ->
-  module_safe L I I safe.
+  module_safe L I I safe se.
 Proof.
   intros SAFE1 SAFE2 COMP. unfold compose in *. unfold option_map in *.
   destruct (link (skel L1) (skel L2)) as [sk|] eqn:Hsk; try discriminate. inv COMP.
   set (L := fun i:bool => if i then L1 else L2).
-  red. intros w se VALID INV.
+  red. intros w VALID INV.
   assert (VALIDSE: forall i, Genv.valid_for (skel (L i)) se).
   destruct i.
   eapply Genv.valid_for_linkorder.
   eapply (link_linkorder _ _ _ Hsk). eauto.
   eapply Genv.valid_for_linkorder.
   eapply (link_linkorder _ _ _ Hsk). eauto.
-  assert (SAFE: forall i, module_safe (L i) I I safe).
+  assert (SAFE: forall i, module_safe (L i) I I safe se).
   destruct i; simpl; auto.
   constructor.
   - intros s t s' REACH STEP.
@@ -159,7 +160,7 @@ Proof.
     + assert (A: safe (L i se) s0). right. left. eauto.
       assert (B: safe (L j se) s'0).
       { inv REACH. subst_dep.
-        generalize (external_safe _ _ _ _ _ _ (SAFE i _ _ (VALIDSE i) INV) s0 q H4 H).
+        generalize (external_safe _ _ _ _ _ _ (SAFE i _ (VALIDSE i) INV) s0 q H4 H).
         intros (wA & SYMBINV & QINV & AFTER).
         eapply initial_safe. eapply SAFE; eauto. eauto. auto. auto. }
       eapply safe_internal;eauto.
@@ -173,9 +174,9 @@ Proof.
       assert (ATEXT: exists q, at_external (L j se) sk0 q).
       eauto.
       destruct ATEXT as (q1 & ATEXT).
-      generalize (external_safe _ _ _ _ _ _ (SAFE j _ _ (VALIDSE j) INV) sk0 q1 H5 ATEXT).
+      generalize (external_safe _ _ _ _ _ _ (SAFE j _ (VALIDSE j) INV) sk0 q1 H5 ATEXT).
       intros (wA & SYMBINV & QINV & AFTER).
-      generalize (final_safe _ _ _ _ _ _ (SAFE i _ _ (VALIDSE i) SYMBINV) _ _ H3 H).
+      generalize (final_safe _ _ _ _ _ _ (SAFE i _ (VALIDSE i) SYMBINV) _ _ H3 H).
       intros VR.
       generalize (AFTER r VR).
       intros ((s' & AFTER1) & C).
@@ -189,17 +190,17 @@ Proof.
     simpl in *. split.
     + (* progress *)
       destruct (valid_query (L1 se) q) eqn: VQ1.
-      * generalize (initial_safe _ _ _ _ _ _ (SAFE true _ _ (VALIDSE true) INV) _ VQ1 SQ).
+      * generalize (initial_safe _ _ _ _ _ _ (SAFE true _ (VALIDSE true) INV) _ VQ1 SQ).
         intros ((s & INIT) & INITSAFE).
         exists (st L true s :: nil). econstructor; eauto.
       * rewrite orb_false_l in VQ.
-        generalize (initial_safe _ _ _ _ _ _ (SAFE false _ _ (VALIDSE false) INV) _ VQ SQ).
+        generalize (initial_safe _ _ _ _ _ _ (SAFE false _ (VALIDSE false) INV) _ VQ SQ).
         intros ((s & INIT) & INITSAFE).
         exists (st L false s :: nil). econstructor; eauto.
     + (* safe *)
       intros s INIT.
       inv INIT.
-      generalize (initial_safe _ _ _ _ _ _ (SAFE i _ _ (VALIDSE i) INV) _ H SQ).
+      generalize (initial_safe _ _ _ _ _ _ (SAFE i _ (VALIDSE i) INV) _ H SQ).
       intros ((s & INIT) & INITSAFE).
       (* repeated work *)
       clear INIT.
@@ -208,7 +209,7 @@ Proof.
       eapply star_refl. constructor.  
   - intros s q REACH EXT. inv EXT.
     eapply reachable_wf_state in REACH. inv REACH. subst_dep.
-    generalize (external_safe _ _ _ _ _ _ (SAFE i _ _ (VALIDSE i) INV) s0 q H3 H).
+    generalize (external_safe _ _ _ _ _ _ (SAFE i _ (VALIDSE i) INV) s0 q H3 H).
     intros (wA & SYMBINV & QINV & AFTER).
     exists wA. split; auto. split; auto.
     intros r SR.
@@ -225,6 +226,50 @@ Proof.
   - intros s r REACH FINAL.
     inv FINAL.
     apply reachable_wf_state in REACH. inv REACH. subst_dep.
-    generalize (final_safe _ _ _ _ _ _ (SAFE i _ _ (VALIDSE i) INV) _ _ H2 H).
+    generalize (final_safe _ _ _ _ _ _ (SAFE i _ (VALIDSE i) INV) _ _ H2 H).
     auto.
 Qed.
+
+(* Relation between two semantics invariants *)
+Record bsim_invariant {li1 li2} (cc: callconv li1 li2) (I1: invariant li1) (I2: invariant li2) : Prop :=
+  { inv_match_symtbl: forall w2 se2 ccw,
+      symtbl_inv I2 w2 se2 ->
+      exists ccw w1 se1, match_senv cc ccw
+        symtbl_inv I1 w1 se1;
+
+    inv_match_query: forall w2 q1 q2 ccw,
+      query_inv I2 w2 q2 ->
+      match_query cc ccw q1 q2 ->
+      exists w1, query_inv I1 w1 q1;
+                       
+    inv_match_reply: forall w2 r1 r2 ccw,
+      reply_inv I2 w2 r2 ->
+      match_reply cc ccw r1 r2 ->
+      exists w1, reply_inv I1 w1 r1;
+
+                      
+  }.
+
+
+(** Safety Preservation Under Backward Simulation *)
+
+Section SAFETY_PRESERVATION.
+
+Context {li1 li2} (cc: callconv li1 li2).
+Context (L1: semantics li1 li1) (L2: semantics li2 li2).
+Context (I1: invariant li1) (I2: invariant li2).
+                 
+Hypothesis BSIM_INV: bsim_invariant cc I1 I2.
+
+Lemma module_safety_preservation:
+    module_safe L1 I1 I1 safe ->
+    backward_simulation cc cc L1 L2 ->
+    module_safe L2 I2 I2 safe.
+Proof.
+  intros SAFE BSIM.
+  inv BSIM. rename X into BSIM.
+  red. intros w2 se2 VSE2 INV2.
+  (* Q1: Can we use the same symtbl to activate the source LTS? *)
+  exploit SAFE. erewrite bsim_skel. eauto.
+  eauto. instantiate (1 := term)
+callconv
